WIP adding ConCert

examples/piggybank/src/piggybank.rs
@@ -1,0 +1,392 @@
+#[cfg(not(feature = "hacspec"))]
+extern crate hacspec_lib;
+
+use hacspec_lib::*;
+
+// #[cfg(feature = "hacspec_attributes")]
+// #[cfg(feature = "hacspec")]
+// use hacspec_attributes::*;
+// #[cfg(not(feature = "hacspec"))]
+// #[cfg(test)]
+// use hacspec_attributes::proof;
+
+#[cfg(test)]
+#[cfg(not(feature = "hacspec"))]
+use creusot_contracts::{ensures, requires};
+
+use hacspec_concordium::*;
+
+#[cfg(not(feature = "hacspec"))]
+/// The state of the piggy bank
+#[derive(Debug, Serialize, PartialEq, Eq)]
+enum PiggyBankState {
+    /// Alive and well, allows for GTU to be inserted.
+    Intact,
+    /// The piggy bank has been emptied, preventing further GTU to be inserted.
+    Smashed,
+}
+
+// Record State :=
+//     build_state { balance : Amount ;
+//                 owner : Address ; 
+//                 piggyState : piggy_bank_state_hacspec_t}.
+/// The state of the piggy bank
+#[derive(Debug, PartialEq, Eq)] // , Serialize
+pub enum PiggyBankStateHacspec {
+    /// Alive and well, allows for GTU to be inserted.
+    Intact,
+    /// The piggy bank has been emptied, preventing further GTU to be inserted.
+    Smashed,
+}
+
+#[cfg(not(feature = "hacspec"))]
+fn coerce_hacspec_to_rust_piggybank_state(pbs : PiggyBankStateHacspec) -> PiggyBankState {
+    match pbs {
+        PiggyBankStateHacspec::Intact  => PiggyBankState::Intact,
+        PiggyBankStateHacspec::Smashed => PiggyBankState::Smashed,
+    }
+}
+
+
+#[cfg(not(feature = "hacspec"))]
+fn coerce_rust_to_hacspec_piggybank_state(pbs : &PiggyBankState) -> PiggyBankStateHacspec {
+    match pbs {
+        PiggyBankState::Intact  => PiggyBankStateHacspec::Intact,
+        PiggyBankState::Smashed => PiggyBankStateHacspec::Smashed,
+    }
+}
+
+pub fn piggy_init_hacspec() -> PiggyBankStateHacspec {
+    // Always succeeds
+    PiggyBankStateHacspec::Intact
+}
+
+// (** We initialize the contract state with [init_value] and set [owner] to the address from which the contract was deployed *)
+// Definition piggyBank_init (chain : Chain) (ctx : ContractCallContext) (_ : Setup) : option State :=
+// Some {| balance := 0 ;
+//         owner := ctx.(ctx_from);
+//         piggyState := Intact |}.
+#[cfg(not(feature = "hacspec"))]
+/// Setup a new Intact piggy bank.
+#[init(contract = "PiggyBank")]
+fn piggy_init(_ctx: &impl HasInitContext) -> InitResult<PiggyBankState> {
+    // Always succeeds
+    Ok(coerce_hacspec_to_rust_piggybank_state(piggy_init_hacspec()))
+}
+
+array!(UserAddress, 32, u8);
+
+#[cfg(not(feature = "hacspec"))]
+fn coerce_rust_to_hacspec_account_address(aa: &AccountAddress) -> UserAddress {
+    UserAddress::from_native_slice(&aa.0)
+}
+
+pub type PiggyInsertResult = Result<(), ()>;
+
+pub fn piggy_insert_hacspec(state: PiggyBankStateHacspec) -> PiggyInsertResult {
+    // Ensure the piggy bank has not been smashed already.
+    match state {
+        PiggyBankStateHacspec::Intact => PiggyInsertResult::Ok(()),
+        PiggyBankStateHacspec::Smashed => PiggyInsertResult::Err(()),
+    }
+}
+
+// Definition insert (n : Amount) (st : State) : State :=
+//     {| balance := st.(balance) + n ;
+//         owner := st.(owner);
+//         piggyState := st.(piggyState) |}.
+#[cfg(not(feature = "hacspec"))]
+/// Insert some GTU into a piggy bank, allowed by anyone.
+#[receive(contract = "PiggyBank", name = "insert", payable)]
+fn piggy_insert<A: HasActions>(
+    _ctx: &impl HasReceiveContext,
+    _amount: Amount,
+    state: &mut PiggyBankState,
+) -> ReceiveResult<A> {
+    // Ensure the piggy bank has not been smashed already.
+    piggy_insert_hacspec(coerce_rust_to_hacspec_piggybank_state(state))?;
+    // Just accept since the GTU balance is managed by the chain.
+    Ok(A::accept())
+}
+
+pub type Context = (UserAddress, UserAddress, u64);
+
+// #[cfg(not(feature = "hacspec"))]
+#[derive(Debug, PartialEq, Eq, Reject)]
+enum SmashError {
+    NotOwner,
+    AlreadySmashed,
+}
+
+#[cfg(not(feature = "hacspec"))]
+fn coerce_rust_to_hacspec_context(ctx: &impl HasReceiveContext) -> Result<Context, SmashError> {
+    Ok((
+        coerce_rust_to_hacspec_account_address(&ctx.owner()),
+        coerce_rust_to_hacspec_account_address(
+            &(match ctx.sender() {
+                Address::Account(a) => Ok(a),
+                _ => Err(SmashError::NotOwner),
+            }?),
+        ),
+        match ctx.self_balance() {
+            Amount { micro_ccd } => micro_ccd,
+        },
+    ))
+}
+
+// enum PiggySmashErr {
+//     OwnerSender,
+//     Smashed,
+// }
+
+type PiggySmashResult = Result<PiggyBankStateHacspec, SmashError>;
+
+// Definition smash (st : State) : State :=
+//     {| balance := 0 ;
+//         owner := st.(owner);
+//         piggyState := Smashed |}.
+fn piggy_smash_hacspec(ctx: Context, state: PiggyBankStateHacspec) -> PiggySmashResult {
+    // Get the contract owner, i.e. the account who initialized the contract.
+    let (owner, sender, _balance) = ctx;
+
+    if !(owner == sender) {
+        PiggySmashResult::Err(SmashError::NotOwner)?;
+    }
+
+    if !(state == PiggyBankStateHacspec::Intact) {
+        PiggySmashResult::Err(SmashError::AlreadySmashed)?;
+    }
+
+    PiggySmashResult::Ok(PiggyBankStateHacspec::Smashed)
+}
+
+#[cfg(not(feature = "hacspec"))]
+/// Smash a piggy bank retrieving the GTU, only allowed by the owner.
+#[receive(contract = "PiggyBank", name = "smash")]
+fn piggy_smash<A: HasActions>(
+    ctx: &impl HasReceiveContext,
+    state: &mut PiggyBankState,
+) -> Result<A, SmashError> {
+    let ctx_hacspec = coerce_rust_to_hacspec_context(ctx)?;
+
+    *state = coerce_hacspec_to_rust_piggybank_state(
+        match piggy_smash_hacspec(ctx_hacspec, coerce_rust_to_hacspec_piggybank_state(state)) {
+            Ok(a) => a,
+            Err(e) => return Err(e),
+        },
+    );
+
+    // Get the current balance of the smart contract.
+    let balance = ctx.self_balance();
+    // Result in a transfer of the whole balance to the contract owner.
+    Ok(A::simple_transfer(&ctx.owner(), balance))
+}
+
+//Tests - type checker ignores #[cfg(test)] parts
+#[cfg(test)]
+extern crate quickcheck;
+#[cfg(test)]
+#[macro_use(quickcheck)]
+extern crate quickcheck_macros;
+
+#[cfg(test)]
+use quickcheck::*;
+
+// Running the initialization ensuring nothing fails and the state of the
+// piggy bank is intact.
+#[cfg(test)]
+#[proof]
+fn test_init_hacspec() -> bool {
+    piggy_init_hacspec() == PiggyBankStateHacspec::Intact
+}
+
+#[cfg(test)]
+#[proof]
+fn test_insert_intact() -> bool {
+    piggy_insert_hacspec(PiggyBankStateHacspec::Intact) == PiggyInsertResult::Ok(())
+}
+
+#[cfg(test)]
+#[proof]
+fn test_insert_smashed() -> bool {
+    piggy_insert_hacspec(PiggyBankStateHacspec::Smashed) == PiggyInsertResult::Err(())
+}
+
+#[cfg(test)]
+#[quickcheck]
+#[proof]
+fn test_smash_intact(owner : UserAddress, balance : u64) -> bool {
+    // Setup the context
+    let sender = owner;
+    let ctx = (owner, sender, balance);
+
+    // Trigger the smash
+    piggy_smash_hacspec(ctx, PiggyBankStateHacspec::Intact) == PiggySmashResult::Ok(PiggyBankStateHacspec::Smashed)
+}
+
+#[cfg(test)]
+#[quickcheck]
+#[proof]
+fn test_smash_intact_not_owner(owner : UserAddress, sender : UserAddress, balance : u64) -> bool{    
+    // Setup the contextt
+    let ctx = (owner, sender, balance);
+
+    // Trigger the smash
+    // TODO: Generate pair of owner sender not equal (not a big issue)
+    owner == sender || piggy_smash_hacspec(ctx, PiggyBankStateHacspec::Intact) == PiggySmashResult::Err(SmashError::NotOwner)
+}
+
+#[cfg(test)]
+#[quickcheck]
+#[proof]
+fn test_smash_smashed(owner : UserAddress, balance : u64) -> bool{
+    // Setup the context
+    let sender = owner;
+    let ctx = (owner, sender, balance);
+
+    // Trigger the smash
+    piggy_smash_hacspec(ctx, PiggyBankStateHacspec::Smashed) == PiggySmashResult::Err(SmashError::AlreadySmashed)
+}
+
+#[cfg(not(feature = "hacspec"))]
+// Unit tests for the smart contract "PiggyBank"
+#[concordium_cfg_test]
+mod tests {
+    use super::*;
+    // Pulling in the testing utils found in concordium_std.
+    use test_infrastructure::*;
+
+    // Running the initialization ensuring nothing fails and the state of the
+    // piggy bank is intact.
+    #[concordium_test]
+    fn test_init() {
+        // Setup
+        let ctx = InitContextTest::empty();
+
+        // Call the init function
+        let state_result = piggy_init(&ctx);
+
+        // Inspect the result
+        let state = state_result.expect_report("Contract initialization failed.");
+
+        claim_eq!(
+            state,
+            PiggyBankState::Intact,
+            "Piggy bank state should be intact after initialization."
+        );
+    }
+
+    #[concordium_test]
+    fn test_insert_intact() {
+        // Setup
+        let ctx = ReceiveContextTest::empty();
+        let amount = Amount::from_micro_ccd(100);
+        let mut state = PiggyBankState::Intact;
+
+        // Trigger the insert
+        let actions_result: ReceiveResult<ActionsTree> = piggy_insert(&ctx, amount, &mut state);
+
+        // Inspect the result
+        let actions = actions_result.expect_report("Inserting GTU results in error.");
+
+        claim_eq!(
+            actions,
+            ActionsTree::accept(),
+            "No action should be produced."
+        );
+        claim_eq!(
+            state,
+            PiggyBankState::Intact,
+            "Piggy bank state should still be intact."
+        );
+    }
+
+    #[concordium_test]
+    fn test_insert_smashed() {
+        // Setup
+        let ctx = ReceiveContextTest::empty();
+        let amount = Amount::from_micro_ccd(100);
+        let mut state = PiggyBankState::Smashed;
+
+        // Trigger the insert
+        let actions_result: ReceiveResult<ActionsTree> = piggy_insert(&ctx, amount, &mut state);
+
+        // Inspect the result
+        claim!(
+            actions_result.is_err(),
+            "Should failed when piggy bank is smashed."
+        );
+    }
+
+    #[concordium_test]
+    fn test_smash_intact() {
+        // Setup the context
+
+        let mut ctx = ReceiveContextTest::empty();
+        let owner = AccountAddress([0u8; 32]);
+        ctx.set_owner(owner);
+        let sender = Address::Account(owner);
+        ctx.set_sender(sender);
+        let balance = Amount::from_micro_ccd(100);
+        ctx.set_self_balance(balance);
+
+        let mut state = PiggyBankState::Intact;
+
+        // Trigger the smash
+        let actions_result: Result<ActionsTree, _> = piggy_smash(&ctx, &mut state);
+
+        // Inspect the result
+        let actions = actions_result.expect_report("Inserting GTU results in error.");
+        claim_eq!(actions, ActionsTree::simple_transfer(&owner, balance));
+        claim_eq!(state, PiggyBankState::Smashed);
+    }
+
+    #[concordium_test]
+    fn test_smash_intact_not_owner() {
+        // Setup the context
+
+        let mut ctx = ReceiveContextTest::empty();
+        let owner = AccountAddress([0u8; 32]);
+        ctx.set_owner(owner);
+        let sender = Address::Account(AccountAddress([1u8; 32]));
+        ctx.set_sender(sender);
+        let balance = Amount::from_micro_ccd(100);
+        ctx.set_self_balance(balance);
+
+        let mut state = PiggyBankState::Intact;
+
+        // Trigger the smash
+        let actions_result: Result<ActionsTree, _> = piggy_smash(&ctx, &mut state);
+
+        let err = actions_result.expect_err_report("Contract is expected to fail.");
+        claim_eq!(
+            err,
+            SmashError::NotOwner,
+            "Expected to fail with error NotOwner"
+        )
+    }
+
+    #[concordium_test]
+    fn test_smash_smashed() {
+        // Setup the context
+        let mut ctx = ReceiveContextTest::empty();
+        let owner = AccountAddress([0u8; 32]);
+        ctx.set_owner(owner);
+        let sender = Address::Account(owner);
+        ctx.set_sender(sender);
+        let balance = Amount::from_micro_ccd(100);
+        ctx.set_self_balance(balance);
+
+        let mut state = PiggyBankState::Smashed;
+
+        // Trigger the smash
+        let actions_result: Result<ActionsTree, _> = piggy_smash(&ctx, &mut state);
+
+        let err = actions_result.expect_err_report("Contract is expected to fail.");
+        claim_eq!(
+            err,
+            SmashError::AlreadySmashed,
+            "Expected  to fail with error AlreadySmashed"
+        )
+    }
+}
