coq/src/Hacspec_Piggybank.v
@@ -6,16 +6,50 @@ Import List.ListNotations.
 Open Scope Z_scope.
 Open Scope bool_scope.
 Open Scope hacspec_scope.
-(* From QuickChick Require Import QuickChick. *)
-(* Require Import QuickChickLib. *)
+From QuickChick Require Import QuickChick.
+Require Import QuickChickLib.
 
 Require Import Hacspec_Lib.
 
 Require Import Hacspec_Concordium.
 
+
+(** * Piggy Bank Contract *)
+(** Implementation of a piggy bank. The contract is based on the Concordium example.
+https://developer.concordium.software/en/mainnet/smart-contracts/tutorials/piggy-bank/writing.html#piggy-bank-writing
+ *)
+From ConCert.Utils Require Import Extras.
+From ConCert.Utils Require Import Automation.
+From ConCert.Execution Require Import Serializable.
+From ConCert.Execution Require Import Blockchain.
+From ConCert.Execution Require Import ContractCommon.
+From Coq Require Import Morphisms ZArith Basics.
+From Coq Require Import List.
+
+(** * Types *)
+
+Import ListNotations.
+Open Scope Z.
+
+Set Nonrecursive Elimination Schemes.
+
+Context {BaseTypes : ChainBase}.
+
+Inductive Msg :=
+| Insert
+| Smash.
+
 Inductive piggy_bank_state_hacspec_t :=
 | Intact : piggy_bank_state_hacspec_t
 | Smashed : piggy_bank_state_hacspec_t.
+
+(** * Types *)
+Record State :=
+    build_state { balance : Amount ;
+                owner : Address ; 
+                piggyState : piggy_bank_state_hacspec_t}.
+
+Definition Setup : Type := unit.
 
 Definition eqb_piggy_bank_state_hacspec_t (x y : piggy_bank_state_hacspec_t) : bool :=
 match x with
@@ -29,25 +63,37 @@ Proof. split. intros; destruct x ; destruct y ; try (f_equal ; apply eqb_leibniz
 Instance eq_dec_piggy_bank_state_hacspec_t : EqDec (piggy_bank_state_hacspec_t) :=
 Build_EqDec (piggy_bank_state_hacspec_t) (eqb_piggy_bank_state_hacspec_t) (eqb_leibniz_piggy_bank_state_hacspec_t).
 
-(* Global Instance show_piggy_bank_state_hacspec_t : Show (piggy_bank_state_hacspec_t) := *)
-(*  @Build_Show (piggy_bank_state_hacspec_t) (fun x => *)
-(*  match x with *)
-(*  Intact => ("Intact")%string *)
-(*  | Smashed => ("Smashed")%string *)
-(*  end). *)
-(* Definition g_piggy_bank_state_hacspec_t : G (piggy_bank_state_hacspec_t) := oneOf_ (returnGen Intact) [returnGen Intact;returnGen Smashed]. *)
-(* Global Instance gen_piggy_bank_state_hacspec_t : Gen (piggy_bank_state_hacspec_t) := Build_Gen piggy_bank_state_hacspec_t g_piggy_bank_state_hacspec_t. *)
+Global Instance show_piggy_bank_state_hacspec_t : Show (piggy_bank_state_hacspec_t) :=
+ @Build_Show (piggy_bank_state_hacspec_t) (fun x =>
+ match x with
+ Intact => ("Intact")%string
+ | Smashed => ("Smashed")%string
+ end).
+Definition g_piggy_bank_state_hacspec_t : G (piggy_bank_state_hacspec_t) := oneOf_ (returnGen Intact) [returnGen Intact;returnGen Smashed].
+Global Instance gen_piggy_bank_state_hacspec_t : Gen (piggy_bank_state_hacspec_t) := Build_Gen piggy_bank_state_hacspec_t g_piggy_bank_state_hacspec_t.
 
+(** We initialize the contract state with [init_value] and set [owner] to the address from which the contract was deployed *)
+Definition piggyBank_init (chain : Chain) (ctx : ContractCallContext) (_ : Setup) : option State :=
+Some {| balance := 0 ;
+        owner := ctx.(ctx_from);
+        piggyState := Intact |}.
 
 Definition piggy_init_hacspec  : piggy_bank_state_hacspec_t :=
   Intact.
 
 Definition user_address_t := nseq (int8) (usize 32).
-(* Instance show_user_address_t : Show (user_address_t) := Build_Show (user_address_t) show. *)
-(* Definition g_user_address_t : G (user_address_t) := arbitrary. *)
-(* Instance gen_user_address_t : Gen (user_address_t) := Build_Gen user_address_t g_user_address_t. *)
+Instance show_user_address_t : Show (user_address_t) := Build_Show (user_address_t) show.
+Definition g_user_address_t : G (user_address_t) := arbitrary.
+Instance gen_user_address_t : Gen (user_address_t) := Build_Gen user_address_t g_user_address_t.
 
 Notation "'piggy_insert_result_t'" := ((result unit unit)) : hacspec_scope.
+
+
+(** * Implementation *)
+Definition insert (n : Amount) (st : State) : State :=
+    {| balance := st.(balance) + n ;
+        owner := st.(owner);
+        piggyState := st.(piggyState) |}.
 
 Definition piggy_insert_hacspec
   (state_0 : piggy_bank_state_hacspec_t)
@@ -59,18 +105,18 @@ Definition piggy_insert_hacspec
 
 Notation "'context_t'" := ((user_address_t ∏ user_address_t ∏ int64
 )) : hacspec_scope.
-(* Instance show_context_t : Show (context_t) := *)
-(* Build_Show context_t (fun x => *)
-(*   let (x, x0) := x in *)
-(*   let (x, x1) := x in *)
-(*   ( *)
-(*     ("(") ++ ((show x) ++ ((",") ++ ((show x0) ++ ((",") ++ ((show x1) ++ (")"))))))))%string. *)
-(* Definition g_context_t : G (context_t) := *)
-(* bindGen arbitrary (fun x0 : user_address_t => *)
-(*   bindGen arbitrary (fun x1 : user_address_t => *)
-(*   bindGen arbitrary (fun x2 : int64 => *)
-(*   returnGen (x0,x1,x2)))). *)
-(* Instance gen_context_t : Gen (context_t) := Build_Gen context_t g_context_t. *)
+Instance show_context_t : Show (context_t) :=
+Build_Show context_t (fun x =>
+  let (x, x0) := x in
+  let (x, x1) := x in
+  (
+    ("(") ++ ((show x) ++ ((",") ++ ((show x0) ++ ((",") ++ ((show x1) ++ (")"))))))))%string.
+Definition g_context_t : G (context_t) :=
+bindGen arbitrary (fun x0 : user_address_t =>
+  bindGen arbitrary (fun x1 : user_address_t =>
+  bindGen arbitrary (fun x2 : int64 =>
+  returnGen (x0,x1,x2)))).
+Instance gen_context_t : Gen (context_t) := Build_Gen context_t g_context_t.
 
 Inductive smash_error_t :=
 | NotOwner : smash_error_t
@@ -88,25 +134,30 @@ Proof. split. intros; destruct x ; destruct y ; try (f_equal ; apply eqb_leibniz
 Instance eq_dec_smash_error_t : EqDec (smash_error_t) :=
 Build_EqDec (smash_error_t) (eqb_smash_error_t) (eqb_leibniz_smash_error_t).
 
-(* Global Instance show_smash_error_t : Show (smash_error_t) := *)
-(*  @Build_Show (smash_error_t) (fun x => *)
-(*  match x with *)
-(*  NotOwner => ("NotOwner")%string *)
-(*  | AlreadySmashed => ("AlreadySmashed")%string *)
-(*  end). *)
-(* Definition g_smash_error_t : G (smash_error_t) := oneOf_ (returnGen NotOwner) [returnGen NotOwner;returnGen AlreadySmashed]. *)
-(* Global Instance gen_smash_error_t : Gen (smash_error_t) := Build_Gen smash_error_t g_smash_error_t. *)
+Global Instance show_smash_error_t : Show (smash_error_t) :=
+ @Build_Show (smash_error_t) (fun x =>
+ match x with
+ NotOwner => ("NotOwner")%string
+ | AlreadySmashed => ("AlreadySmashed")%string
+ end).
+Definition g_smash_error_t : G (smash_error_t) := oneOf_ (returnGen NotOwner) [returnGen NotOwner;returnGen AlreadySmashed].
+Global Instance gen_smash_error_t : Gen (smash_error_t) := Build_Gen smash_error_t g_smash_error_t.
 
 
 Notation "'piggy_smash_result_t'" := ((
   result piggy_bank_state_hacspec_t smash_error_t)) : hacspec_scope.
+
+Definition smash (st : State) : State :=
+    {| balance := 0 ;
+        owner := st.(owner);
+        piggyState := Smashed |}.
 
 Definition piggy_smash_hacspec
   (ctx_1 : context_t)
   (state_2 : piggy_bank_state_hacspec_t)
   : piggy_smash_result_t :=
   let '(owner_3, sender_4, balance_5) :=
-    ctx_1 in 
+    ctx_1 in
   ifbnd negb ((owner_3) array_eq (sender_4)) : bool
   thenbnd (bind (@Err piggy_bank_state_hacspec_t smash_error_t (NotOwner)) (
       fun _ =>  Ok (tt)))
@@ -131,13 +182,13 @@ Definition test_smash_intact
   (balance_7 : int64)
   : bool :=
   let sender_8 : user_address_t :=
-    owner_6 in 
+    owner_6 in
   let ctx_9 : (user_address_t ∏ user_address_t ∏ int64) :=
-    (owner_6, sender_8, balance_7) in 
+    (owner_6, sender_8, balance_7) in
   (piggy_smash_hacspec (ctx_9) (Intact)) =.? (
     @Ok piggy_bank_state_hacspec_t smash_error_t (Smashed)).
-(* QuickChick ( *)
-(*   forAll g_user_address_t (fun owner_6 : user_address_t => forAll g_int64 (fun balance_7 : int64 => test_smash_intact owner_6 balance_7))). *)
+QuickChick (
+  forAll g_user_address_t (fun owner_6 : user_address_t => forAll g_int64 (fun balance_7 : int64 => test_smash_intact owner_6 balance_7))).
 
 Definition test_smash_intact_not_owner
   (owner_10 : user_address_t)
@@ -145,25 +196,241 @@ Definition test_smash_intact_not_owner
   (balance_12 : int64)
   : bool :=
   let ctx_13 : (user_address_t ∏ user_address_t ∏ int64) :=
-    (owner_10, sender_11, balance_12) in 
+    (owner_10, sender_11, balance_12) in
   ((owner_10) array_eq (sender_11)) || ((piggy_smash_hacspec (ctx_13) (
         Intact)) =.? (@Err piggy_bank_state_hacspec_t smash_error_t (
         NotOwner))).
-(* QuickChick ( *)
-(*   forAll g_user_address_t (fun owner_10 : user_address_t => forAll g_user_address_t (fun sender_11 : user_address_t => forAll g_int64 (fun balance_12 : int64 => test_smash_intact_not_owner owner_10 sender_11 balance_12)))). *)
+QuickChick (
+  forAll g_user_address_t (fun owner_10 : user_address_t => forAll g_user_address_t (fun sender_11 : user_address_t => forAll g_int64 (fun balance_12 : int64 => test_smash_intact_not_owner owner_10 sender_11 balance_12)))).
 
 Definition test_smash_smashed
   (owner_14 : user_address_t)
   (balance_15 : int64)
   : bool :=
   let sender_16 : user_address_t :=
-    owner_14 in 
+    owner_14 in
   let ctx_17 : (user_address_t ∏ user_address_t ∏ int64) :=
-    (owner_14, sender_16, balance_15) in 
+    (owner_14, sender_16, balance_15) in
   (piggy_smash_hacspec (ctx_17) (Smashed)) =.? (
     @Err piggy_bank_state_hacspec_t smash_error_t (AlreadySmashed)).
-(* QuickChick ( *)
-(*   forAll g_user_address_t (fun owner_14 : user_address_t => forAll g_int64 (fun balance_15 : int64 => test_smash_smashed owner_14 balance_15))). *)
+QuickChick (
+  forAll g_user_address_t (fun owner_14 : user_address_t => forAll g_int64 (fun balance_15 : int64 => test_smash_smashed owner_14 balance_15))).
+
+
+
+
+
+
+
+Fail 2.
+
+
+
+Definition piggyBank (st : State) (msg : Msg) (ctx : ContractCallContext) : option (State * list ActionBody) :=
+  match msg with
+  | Insert =>
+    if 0 <? ctx.(ctx_amount)
+    then
+      match st with
+      | {| piggyState := Intact |} => Some ((insert ctx.(ctx_amount) st), [])
+      | _ => None 
+      end
+    else None
+  | Smash =>
+    match st with
+    | {| balance := b; owner := o; piggyState := Intact |} => 
+      if address_eqb ctx.(ctx_from) o then (Some ((smash st), [act_transfer o b])) else None
+    | _ => None
+    end
+  end.
+          
+Definition piggyBank_receive (chain : Chain) (ctx : ContractCallContext)
+            (state : State) (msg : option Msg) : option (State * list ActionBody)
+  := match msg with
+      | Some m => piggyBank state m ctx
+      | None => None
+      end.
+
+(* begin hide *)
+(** Deriving the [Serializable] instances for the state and for the messages *)
+Global Instance PiggyState_serializable : Serializable piggy_bank_state_hacspec_t :=
+Derive Serializable piggy_bank_state_hacspec_t_rect<Intact, Smashed>.
+
+Global Instance State_serializable : Serializable State :=
+Derive Serializable State_rect<build_state>.
+
+Global Instance Msg_serializable : Serializable Msg :=
+Derive Serializable Msg_rect<Insert, Smash>.
+(* end hide *)
+
+(** The piggybank contract *)
+Definition piggyBank_contract : Contract Setup Msg State :=
+  build_contract piggyBank_init piggyBank_receive.
+
+
+(** * Proofs *)
+Section FunctionalProperties.
+
+Context {BaseTypes : ChainBase}.
+  
+(** * Functional correctness *)
+Lemma piggybank_correct {prev_state next_state acts msg chain ctx} :
+  prev_state.(piggyState) = Intact -> piggyBank_receive chain ctx prev_state msg = Some (next_state, acts) ->
+  match msg with
+    | Some m => 
+      match m with
+      | Insert => prev_state.(balance) + ctx.(ctx_amount) = next_state.(balance)
+      | Smash => prev_state.(owner) = ctx.(ctx_from) -> next_state.(piggyState) = Smashed /\ 
+        next_state.(balance) = 0 /\ acts = [act_transfer prev_state.(owner) prev_state.(balance)]
+      end
+    | None => False
+  end.
+Proof.
+  intros H1 H2. 
+  unfold piggyBank_receive in H2. 
+  destruct msg; 
+  unfold piggyBank in H2.
+  destruct m.
+  - destruct prev_state. cbn in *. rewrite H1 in H2. unfold insert in *.
+    cbn in H2. destruct (0 <? ctx_amount ctx); try discriminate. inversion H2. cbn. reflexivity.
+  - intros H3. destruct prev_state. cbn in *. rewrite H1 in H2. rewrite H3 in H2. 
+    destruct_address_eq.
+    + inversion H2. cbn. rewrite H3. auto.
+    + discriminate.
+  - discriminate.
+Qed.
+
+End FunctionalProperties.
+
+(** * Safety properties *)
+Section SafetyProperties.
+
+Context {BaseTypes : ChainBase}.
+
+(** ** Owner never changes *)
+Lemma owner_never_changes {prev_state next_state msg chain ctx acts}:
+piggyBank_receive chain ctx prev_state msg = Some (next_state, acts) -> prev_state.(owner) = next_state.(owner).
+Proof.
+  intros H. 
+  unfold piggyBank_receive in H. 
+  destruct msg; unfold piggyBank in H.
+  destruct m; cbn in *; 
+  destruct prev_state; cbn in *; 
+  destruct piggyState0; 
+  destruct (0 <? ctx_amount ctx); try easy.
+  inversion H. cbn in *. reflexivity.
+  - destruct_address_eq; inversion H; auto.
+  - destruct_address_eq; inversion H; auto.
+  - discriminate.  
+Qed.
+
+(** ** Can't change smashed *)
+Lemma cant_change_smashed {prev_state msg chain ctx}:
+  prev_state.(piggyState) = Smashed -> piggyBank_receive chain ctx prev_state msg = None.
+Proof.
+  intros H. 
+  unfold piggyBank_receive. 
+  destruct msg, prev_state; try auto. 
+  cbn in *. unfold piggyBank. 
+  rewrite H. 
+  destruct (0 <? ctx_amount ctx); 
+  now destruct m.
+Qed.
+
+(** ** If piggy bank is intact, balance is only increasing *)
+Lemma if_intact_balance_only_increasing {prev_state next_state chain ctx new_acts}:
+  prev_state.(piggyState) = Intact ->
+  piggyBank_receive chain ctx prev_state (Some Insert) = Some (next_state, new_acts) ->
+  prev_state.(balance) < next_state.(balance).
+Proof.
+  intros H H1. 
+  destruct prev_state. 
+  cbn in *. 
+  rewrite H in H1. 
+  destruct (0 <? ctx_amount ctx) eqn:E; try easy.
+  inversion H1. 
+  cbn in *. 
+  apply Z.ltb_lt in E; Lia.lia.
+Qed. 
+
+(** ** Init total supply correct *)
+Lemma init_total_supply_correct : forall chain ctx setup state,
+  piggyBank_init chain ctx setup = Some state ->
+    state.(balance) = 0.
+Proof.
+  intros; unfold piggyBank_init in H; 
+  now inversion H.
+Qed.
+
+(** ** Balance always positive *)
+Lemma balance_always_positive : forall bstate caddr,
+  reachable bstate ->
+  env_contracts bstate caddr = Some (piggyBank_contract : WeakContract) ->
+  exists cstate,
+    contract_state bstate caddr = Some cstate
+    /\ 0 <= cstate.(balance).
+Proof.
+  intros * reach deployed.
+  apply (lift_contract_state_prop piggyBank_contract); try easy.
+  - cbn. 
+    intros. 
+    apply init_total_supply_correct in H. 
+    Lia.lia.
+  - cbn. intros. 
+    unfold piggyBank_receive in H0. 
+    destruct msg; try easy.
+    unfold piggyBank in H0. 
+    destruct m. 
+    + contract_simpl piggyBank_receive piggyBank_init. 
+      destruct cstate, piggyState0; try easy. 
+      inversion H0. cbn in *. apply Z.ltb_lt in H1. 
+      Lia.lia.
+    + destruct cstate, piggyState0; try easy. 
+      destruct_address_eq; try easy.
+      now inversion H0.
+Qed.
+
+(* (** ** Owner never changes 2 *) *)
+(* Lemma owner_never_changes2 : forall bstate caddr (trace : ChainTrace empty_state bstate), *)
+(*   reachable bstate -> *)
+(*   env_contracts bstate caddr = Some (piggyBank_contract : WeakContract) -> *)
+(*   exists cstate depinfo, *)
+(*     contract_state bstate caddr = Some cstate /\ *)
+(*     deployment_info Setup trace caddr = Some depinfo /\ *)
+(*     depinfo.(deployment_from) = cstate.(owner). *)
+(* Proof. *)
+(*   contract_induction; *)
+(*     intros; auto. *)
+(*     - cbn in *. unfold piggyBank_init in init_some. inversion init_some. easy. *)
+(*     - cbn in *. unfold piggyBank_receive in receive_some. destruct msg; try easy. *)
+(*       unfold piggyBank in receive_some. destruct m; try easy. destruct (0 <? ctx_amount ctx); try easy. *)
+(*       + rewrite IH. destruct prev_state. cbn in *. destruct piggyState0; try easy. inversion receive_some. easy. *)
+(*       + rewrite IH. destruct prev_state. cbn in *. destruct piggyState0; try easy. destruct_address_eq; try easy. *)
+(*       inversion receive_some. easy. *)
+(*     - rewrite IH. cbn in *. unfold piggyBank_receive in receive_some. destruct msg; try easy. *)
+(*       unfold piggyBank in receive_some. destruct m. *)
+(*       + destruct (0 <? ctx_amount ctx); try easy. destruct prev_state. destruct piggyState0; try easy. inversion receive_some. easy. *)
+(*       + destruct prev_state. destruct piggyState0; try easy. destruct_address_eq; try easy. inversion receive_some. easy. *)
+(*     - instantiate (AddBlockFacts := fun _ _ _ _ _ _ => True). *)
+(*       instantiate (DeployFacts := fun _ _ => True). *)
+(*       instantiate (CallFacts := fun _ _ _ _ => True). *)
+(*       unset_all; subst;cbn in *. *)
+(*       destruct_chain_step; auto. *)
+(*       destruct_action_eval; auto. *)
+(* Qed. *)
+End SafetyProperties.
+
+
+
+
+
+
+Fail 2.
+
+
+
+
+
 
 
 
@@ -439,7 +706,6 @@ Module Receive.
           (* #Just (#Pair (mkState False own (tx_amount + bal)) Nil) *)
           (case False : Bool return Maybe Result of
           | False (* Intact *) -> #Just (#Pair (mkState False own (tx_amount + bal)) Nil)
-                              
           (* (* (* (Ok unit unit (tt)) *) *) *)
           | True (* Smashed *) -> #Nothing
           (* (* (* (Err unit unit (tt)) *) *) *)
@@ -560,3 +826,11 @@ End Wrappers.
   
 Definition cf_contract : Contract Setup Msg_coq State_coq :=
   build_contract wrapped_init wrapped_receive.
+
+(* From ConCert.Examples.Counter Require Counter. *)
+From ConCert.Extraction Require Import Common.
+From ConCert.Extraction Require Import ConcordiumExtract.
+From ConCert.Extraction Require Import RustExtract.
+
+Definition COUNTER_MODULE : ConcordiumMod _ _ :=
+  {|  |}.
